src/NLustre/NLCoindSemantics.v
@@ -320,24 +320,24 @@ Module Type NLCOINDSEMANTICS
     -
       assert (nd.(n_name) <> f) as Hnf.
       { intro Hnf. rewrite Hnf in *.
-        apply In_Forall with (2:=find_node_In _ _ _ Hfind) in Hnin.
+        apply Forall_forall with (2:=find_node_In _ _ _ Hfind) in Hnin.
         apply find_node_name in Hfind. auto. }
       econstructor; eauto.
       now apply find_node_other; auto.
       apply Forall_impl_In with (2:=IH).
       intros eq Hin HH. apply HH; clear HH.
       destruct eq; try inversion 1; subst.
-      pose proof (In_Forall _ _ _ Heqs Hin) as Hsem.
+      pose proof Hin as Hsem; apply Forall_forall with (1:=Heqs)in Hsem.
       inversion_clear Hsem as [| ? ? ? ? ? ? ? ? ? ? Hsemn| |].
       inversion_clear Hsemn as [ ? ? ? ? ? Hfind'].
       pose proof (find_node_name _ _ _ Hfind').
       apply find_node_In in Hfind'.
-      apply In_Forall with (1:=Hnin) in Hfind'. auto.
+      apply Forall_forall with (1:=Hnin) in Hfind'. auto.
       take (forall k, _) and specialize (it 0) as Hsem.
       inversion_clear Hsem as [ ? ? ? ? ? Hfind'].
       pose proof (find_node_name _ _ _ Hfind').
       apply find_node_In in Hfind'.
-      apply In_Forall with (1:=Hnin) in Hfind'. auto.
+      apply Forall_forall with (1:=Hnin) in Hfind'. auto.
   Qed.
 
   Lemma sem_equation_cons2:
